<?xml version="1.0" encoding="UTF-8"?>
<rdf:RDF xmlns="http://vast-lab.org/rhdto/"
    xmlns:rdf="http://www.w3.org/1999/02/22-rdf-syntax-ns#"
    xmlns:rdfs="http://www.w3.org/2000/01/rdf-schema#"
    xmlns:crm="http://www.cidoc-crm.org/cidoc-crm/"
    xmlns:crmdig="http://www.ics.forth.gr/isl/CRMdig/"
    xmlns:crmsci="http://www.ics.forth.gr/isl/CRMsci/"
    xmlns:crmpe="http://parthenos.d4science.org/CRMext/CRMpe/"
    xmlns:nont="https://dlnarratives.eu/ontology#">

    <!--
    ========================================================================================
    RHDTO Ontology
    Version 1.1.
    By Achille Felicetti and Franco Niccolucci
    VAST-LAB PIN - 15.09.2025

    Licence: CC BY-NC-SA

    Credit: 
    The present version of this ontology was developed by Achille Felicetti and Franco Niccolucci (ARIADNE RI AISBL and Fondazione PIN), building on previous preliminary and partial work by a wider team of researchers. Use is permitted as long as the present credit statement is visibly and totally included, and it is not for commercial purpose. If you reuse, remix, adapt, rename or anyhow build upon the material, in total or in part, you must license the result under identical terms, and include the present credit statement verbatim.
    ========================================================================================
    -->

    <!--
    This is the RDFS encoding of the RHDT Ontology (RHDTO), a model for cultural heritage based on the concept of digital twin. The ontology is a compatible extension of the CIDOC CRM ISO standard for cultural heritage documentation, and is primarily conceived as a conceptual tool to capture the dual nature of cultural heritage, both tangible and intangible, and to provide, through specific classes and properties, a mechanism for dynamically documenting and analyzing their mutual relationships. It is also designed to model their digital counterparts and the mechanisms that make them interconnected and interoperable, fostering the implementation of complex digital twin systems. The ontology also provides the conceptual tools to describe the reactivity that digital twins are able to deploy for cultural heritage documentation and preservation, by including the semantic description of sensors, signals, activators and all of the process of interacting with real world objects.
    -->

    
    <!-- 
    ////////////////////////////////////////////////////////////////////////////////////////
    //                                                                                    //
    // Classes                                                                            //
    //                                                                                    //
    ////////////////////////////////////////////////////////////////////////////////////////
    -->

    <rdfs:Class rdf:about="http://vast-lab.org/rhdto/HC1_Heritage_Entity">
        <rdfs:subClassOf rdf:resource="http://www.cidoc-crm.org/cidoc-crm/E1_CRM_Entity"/>
        <rdfs:label>HC1 Heritage Entity</rdfs:label>
        <rdfs:comment>This class comprises tangible and intangible entities of the real-world regarded as valuable because of their contribution to society, knowledge and/or culture.</rdfs:comment>
    </rdfs:Class>

    <rdfs:Class rdf:about="http://vast-lab.org/rhdto/HC2_Heritage_Digital_Twin">
        <rdfs:subClassOf rdf:resource="http://www.cidoc-crm.org/cidoc-crm/E89_Propositional_Object"/>
        <rdfs:label>HC2 Heritage Digital Twin</rdfs:label>
        <rdfs:comment>The class consists of the information available in a given system and pertaining to an HC1 Heritage Entity.</rdfs:comment>
    </rdfs:Class>

    <rdfs:Class rdf:about="http://vast-lab.org/rhdto/HC3_Tangible_Entity">
        <rdfs:subClassOf rdf:resource="http://vast-lab.org/rhdto/HC1_Heritage_Entity"/>
        <rdfs:subClassOf rdf:resource="http://www.cidoc-crm.org/cidoc-crm/E18_Physical_Thing"/>
        <rdfs:label>HC3 Tangible Entity</rdfs:label>
        <rdfs:comment>This class comprises tangible, material entities of the real-world, both movable and immovable, regarded as valuable because of their contribution to society, knowledge and/or culture.</rdfs:comment>
    </rdfs:Class>

    <rdfs:Class rdf:about="http://vast-lab.org/rhdto/HC4_Intangible_Aspect">
        <rdfs:subClassOf rdf:resource="http://vast-lab.org/rhdto/HC1_Heritage_Entity"/>
        <rdfs:subClassOf rdf:resource="http://www.cidoc-crm.org/cidoc-crm/E89_Propositional_Object"/>
        <rdfs:label>HC4 Intangible Aspect</rdfs:label>
        <rdfs:comment>This class comprises cultural events, traditions and practices having particular social, historical and cultural significance.</rdfs:comment>
    </rdfs:Class>

    <rdfs:Class rdf:about="http://vast-lab.org/rhdto/HC5_Digital_Representation">
        <rdfs:subClassOf rdf:resource="http://www.ics.forth.gr/isl/CRMdig/D1_Digital_Object"/>
        <rdfs:label>HC5 Digital Representation</rdfs:label>
        <rdfs:comment>This class comprises the digital virtual representations of an HC1 Heritage Entity such as e-texts, images, audio or video items, 3D models, etc.</rdfs:comment>
    </rdfs:Class>

    <rdfs:Class rdf:about="http://vast-lab.org/rhdto/HC6_Digital_Heritage_Document">
        <rdfs:subClassOf rdf:resource="http://vast-lab.org/rhdto/HC5_Digital_Representation"/>
        <rdfs:label>HC6 Digital Heritage Document</rdfs:label>
        <rdfs:comment>This class comprises pieces or collections of digital, non-visual documents, either born-digital or digitised from physical, real-world ones.</rdfs:comment>
    </rdfs:Class>

    <rdfs:Class rdf:about="http://vast-lab.org/rhdto/HC7_Digital_Visual_Object">
        <rdfs:subClassOf rdf:resource="http://vast-lab.org/rhdto/HC5_Digital_Representation"/>
        <rdfs:label>HC7 Digital Visual Object</rdfs:label>
        <rdfs:comment>This class comprises digital visual objects, such as photos and videos, but also special imagery such as X-ray images, spectra of chemical and physical analyses, and so on.</rdfs:comment>
    </rdfs:Class>

    <rdfs:Class rdf:about="http://vast-lab.org/rhdto/HC8_3D_Model">
        <rdfs:subClassOf rdf:resource="http://vast-lab.org/rhdto/HC5_Digital_Representation"/>
        <rdfs:label>HC8 3D Model</rdfs:label>
        <rdfs:comment>This class is used for rendering in detail the 3D model of HC1 Heritage Entity.</rdfs:comment>
    </rdfs:Class>

    <rdfs:Class rdf:about="http://vast-lab.org/rhdto/HC9_Sensor">
        <rdfs:subClassOf rdf:resource="http://www.ics.forth.gr/isl/CRMdig/D8_Digital_Device"/>
        <rdfs:label>HC9 Sensor</rdfs:label>
        <rdfs:comment>This class comprises specialised devices utilised for monitoring and evaluating the conditions of artifacts, structures, or environments of historical significance.</rdfs:comment>
    </rdfs:Class>

    <rdfs:Class rdf:about="http://vast-lab.org/rhdto/HC10_Decider">
        <rdfs:subClassOf rdf:resource="http://parthenos.d4science.org/CRMext/CRMpe/PE1_Service"/>
        <rdfs:label>HC10 Decider</rdfs:label>
        <rdfs:comment>This class comprises software components responsible for receiving signals from sensors and autonomously making decisions aimed at safeguarding cultural objects.</rdfs:comment>
    </rdfs:Class>

    <rdfs:Class rdf:about="http://vast-lab.org/rhdto/HC11_Activator">
        <rdfs:subClassOf rdf:resource="http://www.ics.forth.gr/isl/CRMdig/D8_Digital_Device"/>
        <rdfs:label>HC11 Activator</rdfs:label>
        <rdfs:comment>This class comprises digital devices responsible for executing actions determined by the decider of the digital twin system to safeguard cultural objects.</rdfs:comment>
    </rdfs:Class>

    <rdfs:Class rdf:about="http://vast-lab.org/rhdto/HC12_Signal">
        <rdfs:subClassOf rdf:resource="http://www.ics.forth.gr/isl/CRMdig/D9_Data_Object"/>
        <rdfs:label>HC12 Signal</rdfs:label>
        <rdfs:comment>This class is used to model particular data objects generated by sensors and to document specific detected conditions.</rdfs:comment>
    </rdfs:Class>

    <rdfs:Class rdf:about="http://vast-lab.org/rhdto/HC13_Sensor_Measurement">
        <rdfs:subClassOf rdf:resource="http://www.ics.forth.gr/isl/CRMsci/S21_Measurement"/>
        <rdfs:label>HC13 Sensor Measurement</rdfs:label>
        <rdfs:comment>This class comprises specific measurement events in which a sensor detects and quantifies a specific parameter or condition relevant to the monitoring and conservation of cultural assets.</rdfs:comment>
    </rdfs:Class>

    <rdfs:Class rdf:about="http://vast-lab.org/rhdto/HC14_Activation_Event">
        <rdfs:subClassOf rdf:resource="http://www.cidoc-crm.org/cidoc-crm/E5_Event"/>
        <rdfs:label>HC14 Activation Event</rdfs:label>
        <rdfs:comment>This class serves to model actions performed by an activator to initiate specific interventions or alerts aimed at safeguarding cultural assets.</rdfs:comment>
    </rdfs:Class>

    <rdfs:Class rdf:about="http://vast-lab.org/rhdto/HC15_AI_Component">
        <rdfs:subClassOf rdf:resource="http://www.ics.forth.gr/isl/CRMdig/D14_Software"/>
        <rdfs:label>HC15 AI Component</rdfs:label>
        <rdfs:comment>This class models AI systems within the Heritage Digital Twin, enabling semantic data extraction, adaptive learning, and predictive analysis to enhance knowledge and preservation of cultural heritage.</rdfs:comment>
    </rdfs:Class>

    <rdfs:Class rdf:about="http://vast-lab.org/rhdto/HC16_Simulation_or_Prediction">
        <rdfs:subClassOf rdf:resource="http://www.cidoc-crm.org/cidoc-crm/E5_Event"/>
        <rdfs:label>HC16 Simulation or Prediction</rdfs:label>
        <rdfs:comment>This class represents AI-driven analysis, simulation, and prediction events within the digital twin, enabling scenario testing, forecasting, and decision optimisation for heritage preservation.</rdfs:comment>
    </rdfs:Class>


    <!-- 
    ///////////////////////////////////////////////////////////////////////////////////////
    //
    // Properties
    //
    ///////////////////////////////////////////////////////////////////////////////////////
    -->

    <rdf:Property rdf:about="http://vast-lab.org/rhdto/HP1_has_digital_twin">
        <rdfs:domain rdf:resource="http://vast-lab.org/rhdto/HC1_Heritage_Entity"/>
        <rdfs:range rdf:resource="http://vast-lab.org/rhdto/HC2_Heritage_Digital_Twin"/>
        <rdfs:label>HP1 has digital twin</rdfs:label>
        <rdfs:comment>This property links an instance of HC1 Heritage Entity with an instance of its related HC2 Heritage Digital Twin in a given system.</rdfs:comment>        
    </rdf:Property>

    <rdf:Property rdf:about="http://vast-lab.org/rhdto/HP1i_is_digital_twin_of">
        <rdfs:domain rdf:resource="http://vast-lab.org/rhdto/HC2_Heritage_Digital_Twin"/>
        <rdfs:range rdf:resource="http://vast-lab.org/rhdto/HC1_Heritage_Entity"/>
        <rdfs:label>HP1i is digital twin of</rdfs:label>
        <rdfs:comment>This property indicates that an instance of HC2 Heritage Digital Twin corresponds to an HC1 Heritage Entity.</rdfs:comment>
    </rdf:Property>

    <rdf:Property rdf:about="http://vast-lab.org/rhdto/HP2_has_story">
        <rdfs:domain rdf:resource="http://vast-lab.org/rhdto/HC1_Heritage_Entity"/>
        <rdfs:range rdf:resource="https://dlnarratives.eu/ontology#Narrative"/>
        <rdfs:label>HP2 has story</rdfs:label>
        <rdfs:comment>This property links an instance of HC1 Heritage Entity with an instance of a nont:Narrative that refers to it.</rdfs:comment>        
    </rdf:Property>

    <rdf:Property rdf:about="http://vast-lab.org/rhdto/HP2i_is_story_about">
        <rdfs:domain rdf:resource="https://dlnarratives.eu/ontology#Narrative"/>
        <rdfs:range rdf:resource="http://vast-lab.org/rhdto/HC1_Heritage_Entity"/>
        <rdfs:label>HP2i is story about</rdfs:label>
        <rdfs:comment>This property links a narrative to the HC1 Heritage Entity it describes.</rdfs:comment>
    </rdf:Property>

    <rdf:Property rdf:about="http://vast-lab.org/rhdto/HP3_is_digital_twin_component_of">
        <rdfs:domain rdf:resource="http://vast-lab.org/rhdto/HC2_Heritage_Digital_Twin"/>
        <rdfs:range rdf:resource="http://vast-lab.org/rhdto/HC2_Heritage_Digital_Twin"/>
        <rdfs:label>HP3 is digital twin component of</rdfs:label>
        <rdfs:comment>This property associates an instance of HC2 Heritage Digital Twin with another HC2 of which it is a component.</rdfs:comment>        
    </rdf:Property>

    <rdf:Property rdf:about="http://vast-lab.org/rhdto/HP3i_has_digital_twin_component">
        <rdfs:domain rdf:resource="http://vast-lab.org/rhdto/HC2_Heritage_Digital_Twin"/>
        <rdfs:range rdf:resource="http://vast-lab.org/rhdto/HC2_Heritage_Digital_Twin"/>
        <rdfs:label>HP3i has digital twin component</rdfs:label>
        <rdfs:comment>This property associates an instance of HC2 Heritage Digital Twin with its component parts (also HC2 Heritage Digital Twins).</rdfs:comment>
    </rdf:Property>

    <rdf:Property rdf:about="http://vast-lab.org/rhdto/HP4_narrates">
        <rdfs:domain rdf:resource="https://dlnarratives.eu/ontology#Narration"/>
        <rdfs:range rdf:resource="https://dlnarratives.eu/ontology#Narrative"/>
        <rdfs:label>HP4 narrates</rdfs:label>
        <rdfs:comment>This property links an instance of nont:Narration with an instance of nont:Narrative which has this narration.</rdfs:comment>        
    </rdf:Property>

    <rdf:Property rdf:about="http://vast-lab.org/rhdto/HP4i_is_narrated_by">
        <rdfs:domain rdf:resource="https://dlnarratives.eu/ontology#Narrative"/>
        <rdfs:range rdf:resource="https://dlnarratives.eu/ontology#Narration"/>
        <rdfs:label>HP4i is narrated by</rdfs:label>
        <rdfs:comment>This property identifies the narration (nont:Narration) that contains a given narrative (nont:Narrative).</rdfs:comment>
    </rdf:Property>

    <rdf:Property rdf:about="http://vast-lab.org/rhdto/HP5_has_intangible_aspect">
        <rdfs:domain rdf:resource="http://vast-lab.org/rhdto/HC3_Tangible_Entity"/>
        <rdfs:range rdf:resource="http://vast-lab.org/rhdto/HC4_Intangible_Aspect"/>
        <rdfs:label>HP5 has intangible aspect</rdfs:label>
        <rdfs:comment>This property associates an instance of HC3 Tangible Entity with its intangible aspects (HC4).</rdfs:comment>        
    </rdf:Property>

    <rdf:Property rdf:about="http://vast-lab.org/rhdto/HP5i_is_intangible_aspect_of">
        <rdfs:domain rdf:resource="http://vast-lab.org/rhdto/HC4_Intangible_Aspect"/>
        <rdfs:range rdf:resource="http://vast-lab.org/rhdto/HC3_Tangible_Entity"/>
        <rdfs:label>HP5i is intangible aspect of</rdfs:label>
        <rdfs:comment>This property links an intangible aspect (HC4) to the tangible aspect (HC3) it is associated with.</rdfs:comment>
    </rdf:Property>

    <rdf:Property rdf:about="http://vast-lab.org/rhdto/HP6_has_manifestation_event">
        <rdfs:domain rdf:resource="http://vast-lab.org/rhdto/HC4_Intangible_Aspect"/>
        <rdfs:range rdf:resource="http://www.cidoc-crm.org/cidoc-crm/E5_Event"/>
        <rdfs:subPropertyOf rdf:resource="http://www.cidoc-crm.org/cidoc-crm/P129_is_about"/>
        <rdfs:label>HP6 has manifestation event</rdfs:label>
        <rdfs:comment>This property associates an instance of HC4 Intangible Aspect with the instances of the crm:E5 Event through which the intangible entity manifests itself in the physical world.</rdfs:comment>        
    </rdf:Property>

    <rdf:Property rdf:about="http://vast-lab.org/rhdto/HP6i_is_manifestation_event_of">
        <rdfs:domain rdf:resource="http://www.cidoc-crm.org/cidoc-crm/E5_Event"/>
        <rdfs:range rdf:resource="http://vast-lab.org/rhdto/HC4_Intangible_Aspect"/>
        <rdfs:label>HP6i is manifestation event of</rdfs:label>
        <rdfs:comment>This property is the inverse of HP6, indicating that an event (E5) is the manifestation of an intangible aspect (HC4).</rdfs:comment>
    </rdf:Property>

    <rdf:Property rdf:about="http://vast-lab.org/rhdto/HP7_is_manifestation_of">
        <rdfs:domain rdf:resource="http://vast-lab.org/rhdto/HC3_Tangible_Entity"/>
        <rdfs:range rdf:resource="http://vast-lab.org/rhdto/HC4_Intangible_Aspect"/>
        <rdfs:label>HP7 is manifestation of</rdfs:label>
        <rdfs:comment>This property associates instances of HC3 Tangible Entity with the HC4 Intangible Aspect of which they are the manifestation in the physical world.</rdfs:comment>        
    </rdf:Property>

    <rdf:Property rdf:about="http://vast-lab.org/rhdto/HP7i_is_manifested_by">
        <rdfs:domain rdf:resource="http://vast-lab.org/rhdto/HC4_Intangible_Aspect"/>
        <rdfs:range rdf:resource="http://vast-lab.org/rhdto/HC3_Tangible_Entity"/>
        <rdfs:label>HP7i is manifested by</rdfs:label>
        <rdfs:comment>This property is the inverse of HP7, indicating that an intangible aspect (HC4) is manifested by a tangible aspect (HC3).</rdfs:comment>
    </rdf:Property>

    <rdf:Property rdf:about="http://vast-lab.org/rhdto/HP8_is_narrated_in_document">
        <rdfs:domain rdf:resource="https://dlnarratives.eu/ontology#Narration"/>
        <rdfs:range rdf:resource="http://www.cidoc-crm.org/cidoc-crm/E31_Document"/>
        <rdfs:label>HP8 is narrated in document</rdfs:label>
        <rdfs:comment>This property associates an instance of nont:Narration with instances of E31 Document used to implement it.</rdfs:comment>        
    </rdf:Property>

    <rdf:Property rdf:about="http://vast-lab.org/rhdto/HP8i_document_used_for_narration">
        <rdfs:domain rdf:resource="http://www.cidoc-crm.org/cidoc-crm/E31_Document"/>
        <rdfs:range rdf:resource="https://dlnarratives.eu/ontology#Narration"/>
        <rdfs:label>HP8i document used for narration</rdfs:label>
        <rdfs:comment>This property is the inverse of HP8, linking an E31 Document to the narration (nont:Narration) it implements.</rdfs:comment>
    </rdf:Property>

    <rdf:Property rdf:about="http://vast-lab.org/rhdto/HP9_has_visual_representation">
        <rdfs:domain rdf:resource="http://vast-lab.org/rhdto/HC1_Heritage_Entity"/>
        <rdfs:range rdf:resource="http://vast-lab.org/rhdto/HC7_Digital_Visual_Object"/>
        <rdfs:label>HP9 has visual representation</rdfs:label>
        <rdfs:comment>This property associates an instance of HC1 Heritage Entity with instances of HC7 Digital Visual Object in which it is represented.</rdfs:comment>        
    </rdf:Property>

    <rdf:Property rdf:about="http://vast-lab.org/rhdto/HP9i_is_visual_representation_of">
        <rdfs:domain rdf:resource="http://vast-lab.org/rhdto/HC7_Digital_Visual_Object"/>
        <rdfs:range rdf:resource="http://vast-lab.org/rhdto/HC1_Heritage_Entity"/>
        <rdfs:label>HP9i is visual representation of</rdfs:label>
        <rdfs:comment>This is the inverse of HP9, linking a digital visual object (HC7) to the heritage entity (HC1) it represents.</rdfs:comment>
    </rdf:Property>

    <rdf:Property rdf:about="http://vast-lab.org/rhdto/HP10_tells_about">
        <rdfs:domain rdf:resource="https://dlnarratives.eu/ontology#Narrative"/>
        <rdfs:range rdf:resource="http://www.cidoc-crm.org/cidoc-crm/E5_Event"/>
        <rdfs:label>HP10 tells about</rdfs:label>
        <rdfs:comment>This property is intended to identify the specific events (crm:E5) to which a nont:Narrative relates.</rdfs:comment>        
    </rdf:Property>

    <rdf:Property rdf:about="http://vast-lab.org/rhdto/HP10i_is_told_by">
        <rdfs:domain rdf:resource="http://www.cidoc-crm.org/cidoc-crm/E5_Event"/>
        <rdfs:range rdf:resource="https://dlnarratives.eu/ontology#Narrative"/>
        <rdfs:label>HP10i is told by</rdfs:label>
        <rdfs:comment>This is the inverse of HP10, indicating that an event (E5) is told by a particular narrative (nont:Narrative).</rdfs:comment>
    </rdf:Property>

    <rdf:Property rdf:about="http://vast-lab.org/rhdto/HP11_was_operated_by">
        <rdfs:domain rdf:resource="http://vast-lab.org/rhdto/HC9_Sensor"/>
        <rdfs:range rdf:resource="http://www.ics.forth.gr/isl/CRMdig/D14_Software"/>
        <rdfs:label>HP11 was operated by</rdfs:label>
        <rdfs:comment>This property links an instance of HC9 Sensor to the instances of D14 Software that operate it.</rdfs:comment>        
    </rdf:Property>

    <rdf:Property rdf:about="http://vast-lab.org/rhdto/HP11i_operated">
        <rdfs:domain rdf:resource="http://www.ics.forth.gr/isl/CRMdig/D14_Software"/>
        <rdfs:range rdf:resource="http://vast-lab.org/rhdto/HC9_Sensor"/>
        <rdfs:label>HP11i operated</rdfs:label>
        <rdfs:comment>This is the inverse of HP11, indicating that D14 Software (the operator) operated an HC9 Sensor.</rdfs:comment>
    </rdf:Property>

    <rdf:Property rdf:about="http://vast-lab.org/rhdto/HP12_was_transmitted_to">
        <rdfs:domain rdf:resource="http://vast-lab.org/rhdto/HC12_Signal"/>
        <rdfs:range rdf:resource="http://vast-lab.org/rhdto/HC10_Decider"/>
        <rdfs:label>HP12 was transmitted to</rdfs:label>
        <rdfs:comment>This property associates instances of HC12 Signal with the instances of HC10 Decider, indicating that a certain signal has been transmitted to the digital twin decider for processing.</rdfs:comment>        
    </rdf:Property>

    <rdf:Property rdf:about="http://vast-lab.org/rhdto/HP12i_received">
        <rdfs:domain rdf:resource="http://vast-lab.org/rhdto/HC10_Decider"/>
        <rdfs:range rdf:resource="http://vast-lab.org/rhdto/HC12_Signal"/>
        <rdfs:label>HP12i received</rdfs:label>
        <rdfs:comment>This is the inverse of HP12, indicating that a Decider (HC10) received a Signal (HC12).</rdfs:comment>
    </rdf:Property>

    <rdf:Property rdf:about="http://vast-lab.org/rhdto/HP13_activated">
        <rdfs:domain rdf:resource="http://vast-lab.org/rhdto/HC14_Activation_Event"/>
        <rdfs:range rdf:resource="http://vast-lab.org/rhdto/HC11_Activator"/>
        <rdfs:label>HP13 activated</rdfs:label>
        <rdfs:comment>This property associates the instances of HC14 Activation Event with the instances of HC11 Activator, indicating the specific digital device activated by the digital twin system.</rdfs:comment>        
    </rdf:Property>

    <rdf:Property rdf:about="http://vast-lab.org/rhdto/HP13i_was_activated_by">
        <rdfs:domain rdf:resource="http://vast-lab.org/rhdto/HC11_Activator"/>
        <rdfs:range rdf:resource="http://vast-lab.org/rhdto/HC14_Activation_Event"/>
        <rdfs:label>HP13i was activated by</rdfs:label>
        <rdfs:comment>This is the inverse of HP13, indicating that an activator (HC11) was activated by an activation event (HC14).</rdfs:comment>
    </rdf:Property>

    <rdf:Property rdf:about="http://vast-lab.org/rhdto/HP14_alerted">
        <rdfs:domain rdf:resource="http://vast-lab.org/rhdto/HC14_Activation_Event"/>
        <rdfs:range rdf:resource="http://www.cidoc-crm.org/cidoc-crm/E39_Actor"/>
        <rdfs:label>HP14 alerted</rdfs:label>
        <rdfs:comment>This property associates the instances of HC14 Activation Event with the instances of E39 Actor, indicating the action of alerting human personnel.</rdfs:comment>        
    </rdf:Property>

    <rdf:Property rdf:about="http://vast-lab.org/rhdto/HP14i_was_alerted_by">
        <rdfs:domain rdf:resource="http://www.cidoc-crm.org/cidoc-crm/E39_Actor"/>
        <rdfs:range rdf:resource="http://vast-lab.org/rhdto/HC14_Activation_Event"/>
        <rdfs:label>HP14i was alerted by</rdfs:label>
        <rdfs:comment>This is the inverse of HP14, indicating that an actor (E39) was alerted by an activation event (HC14).</rdfs:comment>
    </rdf:Property>

    <rdf:Property rdf:about="http://vast-lab.org/rhdto/HP15_was_positioned_on">
        <rdfs:domain rdf:resource="http://vast-lab.org/rhdto/HC9_Sensor"/>
        <rdfs:range rdf:resource="http://vast-lab.org/rhdto/HC3_Tangible_Entity"/>
        <rdfs:label>HP15 was positioned on</rdfs:label>
        <rdfs:comment>This property is used to model the spatial relationship between instances of HC9 Sensor and the physical object on which the sensors are located.</rdfs:comment>        
    </rdf:Property>

    <rdf:Property rdf:about="http://vast-lab.org/rhdto/HP15i_hosted">
        <rdfs:domain rdf:resource="http://vast-lab.org/rhdto/HC3_Tangible_Entity"/>
        <rdfs:range rdf:resource="http://vast-lab.org/rhdto/HC9_Sensor"/>
        <rdfs:label>HP15i hosted</rdfs:label>
        <rdfs:comment>This is the inverse of HP15, indicating that a tangible aspect (HC3) hosted a sensor (HC9).</rdfs:comment>
    </rdf:Property>

    <rdf:Property rdf:about="http://vast-lab.org/rhdto/HP16_alerted">
        <rdfs:domain rdf:resource="http://vast-lab.org/rhdto/HC14_Activation_Event"/>
        <rdfs:range rdf:resource="http://www.cidoc-crm.org/cidoc-crm/E39_Actor"/>
        <rdfs:label>HP16 alerted</rdfs:label>
        <rdfs:comment>This property links HC14 Activation Events to E39 Actors, modelling how the digital twin alerts and collaborates with human operators in decision-making processes.</rdfs:comment>
    </rdf:Property>

    <rdf:Property rdf:about="http://vast-lab.org/rhdto/HP16i_was_alerted_by">
        <rdfs:domain rdf:resource="http://www.cidoc-crm.org/cidoc-crm/E39_Actor"/>
        <rdfs:range rdf:resource="http://vast-lab.org/rhdto/HC14_Activation_Event"/>
        <rdfs:label>HP16i was alerted by</rdfs:label>
        <rdfs:comment>This is the inverse of HP16, indicating that an actor (E39) was alerted by an activation event (HC14).</rdfs:comment>
    </rdf:Property>

    <rdf:Property rdf:about="http://vast-lab.org/rhdto/HP17_was_positioned_on">
        <rdfs:domain rdf:resource="http://vast-lab.org/rhdto/HC9_Sensor"/>
        <rdfs:range rdf:resource="http://vast-lab.org/rhdto/HC3_Tangible_Entity"/>
        <rdfs:label>HP17 was positioned on</rdfs:label>
        <rdfs:comment>This property links instances of HC9 Sensors to the pysical cultural object (HC3) they are physically attached to, documenting precise sensor placement on heritage assets.</rdfs:comment>
    </rdf:Property>

    <rdf:Property rdf:about="http://vast-lab.org/rhdto/HP17i_hosted">
        <rdfs:domain rdf:resource="http://vast-lab.org/rhdto/HC3_Tangible_Entity"/>
        <rdfs:range rdf:resource="http://vast-lab.org/rhdto/HC9_Sensor"/>
        <rdfs:label>HP17i hosted</rdfs:label>
        <rdfs:comment>This is the inverse of HP17, indicating that a tangible cultural object (HC3) hosts one or more sensors (HC9).</rdfs:comment>
    </rdf:Property>

    <rdf:Property rdf:about="http://vast-lab.org/rhdto/HP18_uses_algorithm">
        <rdfs:domain rdf:resource="http://vast-lab.org/rhdto/HC15_AI_Component"/>
        <rdfs:range rdf:resource="http://www.ics.forth.gr/isl/CRMdig/D14_Software"/>
        <rdfs:label>HP18 uses algorithm</rdfs:label>
        <rdfs:comment>This property specifies the algorithm (D14) or model used by an AI Component (HC15) to process data and derive insights within the digital twin system.</rdfs:comment>
    </rdf:Property>

    <rdf:Property rdf:about="http://vast-lab.org/rhdto/HP18i_algorithm_is_used_by">
        <rdfs:domain rdf:resource="http://www.ics.forth.gr/isl/CRMdig/D14_Software"/>
        <rdfs:range rdf:resource="http://vast-lab.org/rhdto/HC15_AI_Component"/>
        <rdfs:label>HP18i algorithm is used by</rdfs:label>
        <rdfs:comment>This is the inverse of HP18, indicating the algorithm used by the AI component to perform its operations.</rdfs:comment>
    </rdf:Property>

    <rdf:Property rdf:about="http://vast-lab.org/rhdto/HP19_was_trained_using">
        <rdfs:domain rdf:resource="http://vast-lab.org/rhdto/HC15_AI_Component"/>
        <rdfs:range rdf:resource="http://www.cidoc-crm.org/cidoc-crm/E31_Document"/>
        <rdfs:label>HP19 was trained using</rdfs:label>
        <rdfs:comment>This property identifies the training data, protocols, or datasets used to teach the AI Component, supporting its learning, prediction, and performance in heritage-related tasks.</rdfs:comment>
    </rdf:Property>

<rdf:Property rdf:about="http://vast-lab.org/rhdto/HP19i_was_used_for_training">
        <rdfs:domain rdf:resource="http://www.cidoc-crm.org/cidoc-crm/E31_Document"/>
        <rdfs:range rdf:resource="http://vast-lab.org/rhdto/HC15_AI_Component"/>
        <rdfs:label>HP19i was used for training</rdfs:label>
        <rdfs:comment>This is the inverse of HP19, indicating the documentation used for training an AI Component (HC15)</rdfs:comment>
    </rdf:Property>

</rdf:RDF>